src/lib/data/Kuiper.Bitmask.fsti
@@ -3,21 +3,41 @@ module Kuiper.Bitmask
 open Kuiper
 #lang-pulse
 
+module U32 = FStar.UInt32
+
+val bitmask_len (n : nat) : (nb : nat{nb * 32 >= n})
+
 val bitmask (n:nat) : Type0
 
-val bitmask_pts_to (#n:_) (b:bitmask n) (p : FStar.GSet.set nat)
+val bitmask_pts_to (#n:_) (b:bitmask n) (p : GSet.set nat)
   : slprop
 
-fn alloc (n:nat)
-  requires emp
+
+fn init_empty (n:nat) (a : larray u32 (bitmask_len n))
+  requires
+    exists* v_a.
+      a |-> v_a **
+      pure (forall i. v_a @! i == 0ul)
   returns  b : bitmask n
-  ensures  bitmask_pts_to b FStar.GSet.empty
+  ensures  bitmask_pts_to b GSet.empty
+
+
+let full #a : GSet.set a = GSet.comprehend (fun _ -> true)
+let full_mask = U32.uint_to_t 0xffffffff
+
+fn init_full (n:nat) (a : larray u32 (bitmask_len n))
+  requires
+    exists* v_a.
+      a |-> v_a **
+      pure (forall i. v_a @! i == full_mask)
+  returns  b : bitmask n
+  ensures  bitmask_pts_to b full
 
 fn get (#n:nat) (b:bitmask n) (i:sz) (#p : GSet.set nat)
   preserves bitmask_pts_to b p
   requires  pure (i < n)
   returns   v : bool
-  ensures   pure (v = FStar.GSet.mem (SizeT.v i) p)
+  ensures   pure (v = GSet.mem (SizeT.v i) p)
 
 let add #a (x:a) (s: GSet.set a) : GSet.set a =
   GSet.union (GSet.singleton x) s
@@ -25,9 +45,12 @@ let add #a (x:a) (s: GSet.set a) : GSet.set a =
 let remove #a (x:a) (s: GSet.set a) : GSet.set a =
   GSet.intersect (GSet.complement (GSet.singleton x)) s
 
-fn set (#n:nat) (b:bitmask n) (i:sz) (v:bool) (#p : GSet.set nat)
+fn set (#n:nat) (b:bitmask n) (i:sz) (#p : GSet.set nat)
   requires  bitmask_pts_to b p
   requires  pure (i < n)
-  ensures   exists* p'.
-              bitmask_pts_to b p' ** 
-                pure (p' == (if v then add (SizeT.v i) p else remove (SizeT.v i) p))
+  ensures   bitmask_pts_to b (add (SizeT.v i) p) 
+
+fn unset (#n:nat) (b:bitmask n) (i:sz) (#p : GSet.set nat)
+  requires  bitmask_pts_to b p
+  requires  pure (i < n)
+  ensures   bitmask_pts_to b (remove (SizeT.v i) p)
