src/lib/data/Kuiper.Bitmask.fst
@@ -1,0 +1,288 @@
+module Kuiper.Bitmask
+#set-options "--debug SMTFail --split_queries always"
+
+open Kuiper
+module U32 = FStar.UInt32
+module SZ = Kuiper.SizeT
+module UI = FStar.UInt
+#lang-pulse
+
+
+let getBit (u : u32) (i : szlt 32sz) : bool
+= U32.shift_right u (SZ.sizet_to_u32 i) `U32.logand` 1ul = 1ul
+
+let setBit (u : u32) (i : szlt 32sz) : u32
+= u `U32.logor` U32.shift_left 1ul (SZ.sizet_to_u32 i) 
+
+let unsetBit (u : u32) (i : szlt 32sz) : u32
+= u `U32.logand` U32.lognot (U32.shift_left 1ul (SZ.sizet_to_u32 i))
+
+let lemma_nth_1 ()
+: Lemma (requires true) (ensures forall (i : natlt 31). UI.nth #32 1 i == false)
+=
+  introduce forall (i : natlt 31). UI.nth #32 1 i == false
+  with (
+    assert UI.to_vec #31 (1 / 2) `FStar.Seq.equal` UI.to_vec (UI.zero 31);
+    UI.zero_to_vec_lemma #31 i
+  )
+
+let shift_bit_lemma_true (u : UI.uint_t 32) (i : natlt 32)
+: Lemma
+    (requires true)
+    (ensures UI.nth #32 (UI.shift_right #32 u i `UI.logand` 1) 31 == UI.nth #32 u (31 - i))
+=
+  UI.shift_right_lemma_2 u i i;
+  UI.logand_definition (UI.shift_right #32 u i) 1 31
+
+let shift_bit_lemma_false (u : UI.uint_t 32)
+: Lemma
+    (requires true)
+    (ensures forall (i : natlt 31). UI.nth #32 (u `UI.logand` 1) i == false)
+=
+  lemma_nth_1 ()
+
+let cmp_1_lemma (u : UI.uint_t 32)
+: Lemma
+    (requires forall (i : natlt 31). UI.nth u i == false)
+    (ensures UI.nth #32 u 31 == (u = 1))
+=
+  if UI.nth #32 u 31
+    then (
+      lemma_nth_1 ();
+      UI.nth_lemma u 1
+    )
+    else ()
+
+let getBit_lemma (u : u32) (i : szlt 32)
+: Lemma
+    (requires true)
+    (ensures getBit u i == UI.nth #32 u (31 - i))
+=
+  shift_bit_lemma_true u i;
+  shift_bit_lemma_false (UI.shift_right #32 u i);
+  cmp_1_lemma (UI.shift_right #32 u i `UI.logand` 1);
+  ()
+
+let shift_left_1_lemma_false (i j : szlt 32)
+: Lemma
+    (requires SZ.v j <> 31 - i)
+    (ensures UI.nth #32 (UI.shift_left 1 i) j == false)
+=
+  if (j >= 32 - i)
+    then ()
+    else lemma_nth_1 ()
+
+let setBit_lemma_ensures (u : u32) (i : szlt 32)
+: Lemma
+    (requires true)
+    (ensures UI.nth #32 (setBit u i) (31 - i))
+= ()
+
+
+let setBit_lemma_preserves (u : u32) (i j : szlt 32)
+: Lemma
+    (requires j <> i)
+    (ensures UI.nth #32 (setBit u i) (31 - j) = UI.nth #32 u (31 - j))
+=
+  shift_left_1_lemma_false i (31sz -^ j)
+  
+let unsetBit_lemma_ensures (u : u32) (i : szlt 32)
+: Lemma
+    (requires true)
+    (ensures UI.nth #32 (unsetBit u i) (31 - i) == false)
+=
+  UI.shift_left_lemma_2 #32 1 i (31 - i);
+  UI.lognot_definition (UI.shift_left #32 1 i) (31 - i);
+  UI.logand_definition u (UI.lognot (UI.shift_left #32 1 i)) (31 - i);
+  ()
+
+let unsetBit_lemma_preserves (u : u32) (i j : szlt 32)
+: Lemma
+    (requires j <> i)
+    (ensures UI.nth #32 (unsetBit u i) (31 - j) = UI.nth #32 u (31 - j))
+=
+  shift_left_1_lemma_false i (31sz -^ j)
+
+let bitmask_len (n : nat) = (n + 31) / 32
+noeq
+type bitmask (n : nat) : Type0 =
+  | BM of larray u32 (bitmask_len n)
+
+let core #n (BM a : bitmask n) = a
+
+
+let bitmask_pts_to (#n:_) (b:bitmask n) (p : GSet.set nat)
+: slprop
+= 
+  exists* (a : lseq u32 (bitmask_len n)).
+    core b |-> a **
+    pure (
+      forall (i : szlt n).
+        (GSet.mem (SZ.v i) p = getBit (a @! (i / 32)) (i %^ 32sz))
+    )
+
+fn init_empty (n:nat) (a : larray u32 (bitmask_len n))
+  requires
+    exists* v_a.
+      a |-> v_a **
+      pure (forall i. v_a @! i == 0ul)
+  returns  b : bitmask n
+  ensures  bitmask_pts_to b GSet.empty
+{
+  let b : bitmask n = BM a;
+  assert rewrites_to a (core b);
+  Pulse.Lib.Array.pts_to_len a;
+  fold bitmask_pts_to b GSet.empty;
+  b;
+}
+
+let getBit_lemma_full_mask ()
+: Lemma
+  (requires true)
+  (ensures forall (i : szlt 32). getBit full_mask i == true)
+= 
+  introduce forall (i : szlt 32). getBit full_mask i == true
+  with getBit_lemma full_mask i
+
+
+fn init_full (n:nat) (a : larray u32 (bitmask_len n))
+  requires
+    exists* v_a.
+      a |-> v_a **
+      pure (forall i. v_a @! i == (U32.uint_to_t 0xffffffff))
+  returns  b : bitmask n
+  ensures  bitmask_pts_to b full
+{
+  let b : bitmask n = BM a;
+  assert rewrites_to a (core b);
+  Pulse.Lib.Array.pts_to_len a;
+  with va. assert a |-> va;
+
+  assert pure (forall (i : szlt n). va @! i / 32 == full_mask);
+  getBit_lemma_full_mask ();
+
+  fold bitmask_pts_to b full;
+  b 
+}
+
+fn get (#n:nat) (b:bitmask n) (i:sz) (#p : GSet.set nat)
+  preserves bitmask_pts_to b p
+  requires  pure (i < n)
+  returns   v : bool
+  ensures   pure (v = GSet.mem (SZ.v i) p)
+{
+  unfold bitmask_pts_to;
+
+  open Pulse.Lib.Array;
+  let word = (core b).(i /^ 32sz);
+  let bit = i %^ 32sz;
+
+  let v : bool = getBit word bit;
+  getBit_lemma word bit;
+
+  fold bitmask_pts_to b p;
+
+  v;
+}
+
+let rem_lemma_not_eq (i j : nat) (n : pos)
+: Lemma (requires i <> j /\ i / n == j / n) (ensures i % n <> j % n)
+= ()
+
+let set_lemma_preserves (#n : nat) (a : lseq u32 (bitmask_len n)) (i : szlt n)
+: Lemma
+  (requires true)
+  (ensures forall (j : szlt n). j <> i ==>
+    getBit (Seq.upd a (i / 32) (setBit (a @! i / 32) (i %^ 32sz)) @! j / 32) (j %^ 32sz) ==
+    getBit (a @! j / 32) (j %^ 32sz)
+  )
+= 
+  introduce forall (j : szlt n). j <> i ==>
+    getBit (Seq.upd a (i / 32) (setBit (a @! i / 32) (i %^ 32sz)) @! j / 32) (j %^ 32sz) ==
+    getBit (a @! j / 32) (j %^ 32sz)
+  with (
+    if (i = j) then () else
+    let word = a @! i / 32 in
+    let word' = setBit word (i %^ 32sz) in
+    if (i / 32 = j / 32)
+      then (
+        rem_lemma_not_eq i j 32;
+        setBit_lemma_preserves word (i %^ 32sz) (j %^ 32sz);
+        getBit_lemma word (j %^ 32sz);
+        getBit_lemma word' (j %^ 32sz)
+      )
+      else Seq.lemma_index_upd2 a (i / 32) word' (j / 32)
+  )
+
+let unset_lemma_preserves (#n : nat) (a : lseq u32 (bitmask_len n)) (i : szlt n)
+: Lemma
+  (requires true)
+  (ensures forall (j : szlt n). j <> i ==>
+    getBit (Seq.upd a (i / 32) (unsetBit (a @! i / 32) (i %^ 32sz)) @! j / 32) (j %^ 32sz) ==
+    getBit (a @! j / 32) (j %^ 32sz)
+  )
+= 
+  introduce forall (j : szlt n). j <> i ==>
+    getBit (Seq.upd a (i / 32) (unsetBit (a @! i / 32) (i %^ 32sz)) @! j / 32) (j %^ 32sz) ==
+    getBit (a @! j / 32) (j %^ 32sz)
+  with (
+    if (i = j) then () else
+    let word = a @! i / 32 in
+    let word' = unsetBit word (i %^ 32sz) in
+    if (i / 32 = j / 32)
+      then (
+        rem_lemma_not_eq i j 32;
+        unsetBit_lemma_preserves word (i %^ 32sz) (j %^ 32sz);
+        getBit_lemma word (j %^ 32sz);
+        getBit_lemma word' (j %^ 32sz);
+        ()
+      )
+      else Seq.lemma_index_upd2 a (i / 32) word' (j / 32)
+  )
+  
+
+fn set (#n:nat) (b:bitmask n) (i:sz) (#p : GSet.set nat)
+  requires  bitmask_pts_to b p
+  requires  pure (i < n)
+  ensures   bitmask_pts_to b (add (SZ.v i) p) 
+{
+  unfold bitmask_pts_to;
+
+  with a. assert core b |-> a;
+
+  open Pulse.Lib.Array;
+  let word = (core b).(i /^ 32sz);
+  let bit = i %^ 32sz;
+
+  let word' = setBit word bit;
+  (core b).(i /^ 32sz) <- word';
+
+  setBit_lemma_ensures word bit;
+  getBit_lemma word' bit;
+  set_lemma_preserves a i;
+
+  fold bitmask_pts_to b (add (SZ.v i) p);
+}
+
+fn unset (#n:nat) (b:bitmask n) (i:sz) (#p : GSet.set nat)
+  requires  bitmask_pts_to b p
+  requires  pure (i < n)
+  ensures   bitmask_pts_to b (remove (SizeT.v i) p)
+{
+  unfold bitmask_pts_to;
+
+  with a. assert core b |-> a;
+
+  open Pulse.Lib.Array;
+  let word = (core b).(i /^ 32sz);
+  let bit = i %^ 32sz;
+
+  let word' = unsetBit word bit;
+  (core b).(i /^ 32sz) <- word';
+
+  unsetBit_lemma_ensures word bit;
+  getBit_lemma word' bit;
+  unset_lemma_preserves a i;
+
+  fold bitmask_pts_to b (remove (SZ.v i) p);
+}
